remove unused commutativity proofs

commutativity.thy
@@ -10,837 +10,9 @@ begin
 text \<open>This theory proves commutativity between certain actions in executions.\<close>
 
 
-
-definition commutativeS :: "('proc::valueType, 'ls, 'operation, 'any::valueType) state \<Rightarrow> invocId \<times> ('proc, 'operation, 'any) action \<Rightarrow> invocId \<times> ('proc, 'operation, 'any) action \<Rightarrow> bool" where
-  "commutativeS s a b \<equiv> (\<forall>t. ((s ~~ [a,b] \<leadsto>*  t) \<longleftrightarrow> (s ~~ [b,a] \<leadsto>* t)))"
-
-
-lemma useCommutativeS:
-  assumes "commutativeS s a b"
-  shows "(s ~~ [a,b] \<leadsto>*  t) \<longleftrightarrow> (s ~~ [b,a] \<leadsto>* t)"
-  using assms by (simp add: commutativeS_def)
-
-
-definition "precondition a C \<equiv> \<exists>C'. C ~~ a \<leadsto> C'"
-
-lemma usePrecondition: "precondition a C \<Longrightarrow> \<exists>C'. C ~~ a \<leadsto> C'"
-  by (simp add: precondition_def)
-
-lemma usePrecondition2: "precondition a C \<Longrightarrow> (\<And>C'. C ~~ a \<leadsto> C' \<Longrightarrow> P C') \<Longrightarrow> \<exists>C'. (C ~~ a \<leadsto> C') \<and> P C'"
-  using usePrecondition by blast
-
-lemma commutativeS_switchArgs: 
-  "commutativeS s a b \<longleftrightarrow> commutativeS s b a"
-  by (auto simp add: commutativeS_def)
-
-
-lemma preconditionI: "\<lbrakk>s ~~ a \<leadsto> B\<rbrakk> \<Longrightarrow> precondition a s"
-  by (auto simp add: precondition_def)
-
-lemma show_commutativeS[case_names preAB preBA commute ]: 
-  assumes a1:  "\<And>s1 s2. \<lbrakk>s ~~ a \<leadsto> s1; s1 ~~ b \<leadsto> s2\<rbrakk> \<Longrightarrow> \<exists>s1. (s ~~ b \<leadsto> s1) \<and> (\<exists>s2. s1 ~~ a \<leadsto> s2)" 
-    and a2:  "\<And>s1 s2. \<lbrakk>s ~~ b \<leadsto> s1; s1 ~~ a \<leadsto> s2\<rbrakk> \<Longrightarrow> \<exists>s1. (s ~~ a \<leadsto> s1) \<and> (\<exists>s2. s1 ~~ b \<leadsto> s2)" 
-    and a4:  "\<And>s1 s2 s1' s2'. \<lbrakk>s ~~ a \<leadsto> s1; s1 ~~ b \<leadsto> s2; s ~~ b \<leadsto> s1'; s1' ~~ a \<leadsto> s2'\<rbrakk> \<Longrightarrow> s2 = s2'"
-  shows "commutativeS s a b"
-  by (auto simp add: commutativeS_def  steps_appendFront,
-      insert a1 a4, blast,
-      insert a2 a4, blast)
-
-lemma show_commutativeS_pres[case_names preBfront preAfront preAback preBback commute ]: 
-  assumes a1:  "\<And>s1. \<lbrakk>s ~~ a \<leadsto> s1; precondition b s1\<rbrakk> \<Longrightarrow> precondition b s"
-    and a1': "\<And>s1. \<lbrakk>s ~~ b \<leadsto> s1; precondition a s1\<rbrakk> \<Longrightarrow> precondition a s"
-    and a2:  "\<And>s1. \<lbrakk>s ~~ b \<leadsto> s1; precondition a s\<rbrakk> \<Longrightarrow> precondition a s1"
-    and a2': "\<And>s1. \<lbrakk>s ~~ a \<leadsto> s1; precondition b s\<rbrakk> \<Longrightarrow> precondition b s1"
-    and a4:  "\<And>s1 s2 s1' s2'. \<lbrakk>s ~~ a \<leadsto> s1; s1 ~~ b \<leadsto> s2; s ~~ b \<leadsto> s1'; s1' ~~ a \<leadsto> s2'\<rbrakk> \<Longrightarrow> s2 = s2'"
-  shows "commutativeS s a b"
-proof (auto simp add: commutativeS_def precondition_def steps_appendFront steps_empty; rule usePrecondition2)
-  show "precondition b s"
-    if c0: "s ~~ a \<leadsto> B"
-      and c1: "B ~~ b \<leadsto> t"
-    for  t B
-    using a1 c0 c1 preconditionI by blast
-
-  show "Ba ~~ a \<leadsto> t"
-    if c0: "s ~~ a \<leadsto> B"
-      and c1: "B ~~ b \<leadsto> t"
-      and c2: "s ~~ b \<leadsto> Ba"
-    for  t B Ba
-    by (metis a2 a4 c0 c1 c2 preconditionI usePrecondition)
-
-  show "precondition a s"
-    if c0: "s ~~ b \<leadsto> B"
-      and c1: "B ~~ a \<leadsto> t"
-    for  t B
-    using a1' c0 c1 preconditionI by blast
-
-  show "Ba ~~ b \<leadsto> t"
-    if c0: "s ~~ b \<leadsto> B"
-      and c1: "B ~~ a \<leadsto> t"
-      and c2: "s ~~ a \<leadsto> Ba"
-    for  t B Ba
-    by (metis a2' a4 c0 c1 c2 preconditionI usePrecondition)
-qed
-
-
-definition differentIds :: "(invocId \<times> ('proc, 'operation, 'any) action) \<Rightarrow> (invocId \<times> ('proc, 'operation, 'any) action) \<Rightarrow> bool" where
-  "differentIds a b \<equiv> case (a,b) of
-   ((s1, ANewId u1), (s2, ANewId u2)) \<Rightarrow> (u1 \<noteq> u2)
- | ((s1, ABeginAtomic u1 nt1), (s2, ABeginAtomic u2 nt2)) \<Rightarrow> (u1 \<noteq> u2)
- | ((s1, ADbOp u1 o1 r1), (s2, ADbOp u2 o2 r2)) \<Rightarrow> (u1 \<noteq> u2)
- | _ \<Rightarrow> True"
-
-lemma differentIds_newId:
-  "differentIds (s1, ANewId u1) (s2, ANewId u2) \<longleftrightarrow> (u1 \<noteq> u2)"
-  by (simp add: differentIds_def)
-
-lemma differentIds_beginAtomic:
-  "differentIds (s1, ABeginAtomic u1 nt1) (s2, ABeginAtomic u2 nt2) \<longleftrightarrow> (u1 \<noteq> u2)"
-  by (simp add: differentIds_def)
-
-lemma differentIds_dbop:
-  "differentIds (s1, ADbOp u1 o1 r1) (s2, ADbOp u2 o2 r2) \<longleftrightarrow> (u1 \<noteq> u2)"
-  by (simp add: differentIds_def)
-
-lemma steps_to_differentIds: 
-  assumes step1: "s ~~ (sa,a) \<leadsto> B" and step2: "B ~~ (sb,b) \<leadsto> t"
-  shows "differentIds (sa,a) (sb,b)"
-  by (cases a; cases b;
-      insert step1 step2,
-      auto simp add: differentIds_def step_simps split: if_splits)
-
-lemma steps_to_differentIds2: 
-  assumes step1: "s ~~ a \<leadsto> B" and step2: "B ~~ b \<leadsto> t"
-  shows "differentIds a b"
-  by (metis prod.swap_def step1 step2 steps_to_differentIds swap_swap)
-
-lemma differentIds_commute: 
-  shows "differentIds a b = differentIds b a"
-  by (auto simp add: differentIds_def split: action.splits)
-
-
-lemma show_commutativeS_pres2[case_names preBfront preAfront preAback preBback commute ]: 
-  assumes a1:  "\<And>s1. \<lbrakk>s ~~ a \<leadsto> s1; precondition b s1; differentIds a b\<rbrakk> \<Longrightarrow> precondition b s"
-    and a1': "\<And>s1. \<lbrakk>s ~~ b \<leadsto> s1; precondition a s1; differentIds a b\<rbrakk> \<Longrightarrow> precondition a s"
-    and a2:  "\<And>s1. \<lbrakk>s ~~ b \<leadsto> s1; precondition a s; differentIds a b\<rbrakk> \<Longrightarrow> precondition a s1"
-    and a2': "\<And>s1. \<lbrakk>s ~~ a \<leadsto> s1; precondition b s; differentIds a b\<rbrakk> \<Longrightarrow> precondition b s1"
-    and a4:  "\<And>s1 s2 s1' s2'. \<lbrakk>s ~~ a \<leadsto> s1; s1 ~~ b \<leadsto> s2; s ~~ b \<leadsto> s1'; s1' ~~ a \<leadsto> s2'\<rbrakk> \<Longrightarrow> s2 = s2'"
-  shows "commutativeS s a b"
-proof (auto simp add: commutativeS_def precondition_def steps_appendFront steps_empty)
-  fix t B
-  assume step1: "s ~~ a \<leadsto> B" and step2: "B ~~ b \<leadsto> t"
-
-  then have dIds: "differentIds a b"
-    using steps_to_differentIds2 by blast
-
-  show "\<exists>B. (s ~~ b \<leadsto> B) \<and> (B ~~ a \<leadsto> t)"
-    by (metis a1 a2 a4 dIds preconditionI step1 step2 usePrecondition)
-next   
-  fix t B
-  assume step1: "s ~~ b \<leadsto> B" and step2: "B ~~ a \<leadsto> t"
-
-  then have dIds: "differentIds a b"
-    using steps_to_differentIds2
-    using differentIds_commute by blast 
-
-  show "\<exists>B. (s ~~ a \<leadsto> B) \<and> (B ~~ b \<leadsto> t)"
-    by (metis a1' a2' a4 dIds preconditionI step1 step2 usePrecondition)
-qed  
-
-
-lemma precondition_alocal:
-  "precondition (s, ALocal) C = (\<exists>ls f ls'. localState C s \<triangleq> ls \<and> currentProc C s \<triangleq> f \<and> f ls = LocalStep ls')"
-  by (auto simp add: precondition_def intro: step.intros elim: step_elims)
-
-
-lemma precondition_newid:
-  "precondition (s, ANewId uid) C = (\<exists>ls f ls' ls''.
-     localState C s \<triangleq> ls \<and> currentProc C s \<triangleq> f \<and> f ls = NewId ls' 
-   \<and>  generatedIds C (to_nat uid) = None \<and> uniqueIds uid = {to_nat uid} 
-   \<and>  ls' uid \<triangleq> ls'')"
-  by (auto simp add: precondition_def intro: step.intros elim!: step_elims)
-
-
-lemma precondition_beginAtomic:
-  "precondition (s, ABeginAtomic tx snapshot) C = 
-    (\<exists>ls f ls' vis. 
-        localState C s \<triangleq> ls 
-      \<and> currentProc C s \<triangleq> f 
-      \<and> f ls = BeginAtomic ls' 
-      \<and> currentTransaction C s = None 
-      \<and> transactionStatus C tx = None
-      \<and> visibleCalls C s \<triangleq> vis
-      \<and> chooseSnapshot snapshot vis C)"
-  by (auto simp add: precondition_def step_simps )
-
-lemma precondition_endAtomic:
-  "precondition (s, AEndAtomic) C = (\<exists>ls f ls'. localState C s \<triangleq> ls \<and> currentProc C s \<triangleq> f \<and> f ls = EndAtomic ls' \<and> currentTransaction C s \<noteq> None)"
-  by (auto simp add: precondition_def intro: step.intros elim!: step_elims)
-
-lemma precondition_invoc:
-  "precondition (s, AInvoc proc) C = (localState C s = None \<and> uniqueIds proc \<subseteq> knownIds C \<and> invocationOp C s = None)"
-  by (auto simp add: precondition_def step.simps)
-
-
-lemma precondition_dbop:
-  "precondition (s, ADbOp c operation  res) C = (\<exists>ls f ls' t vis. calls C c = None \<and> localState C s \<triangleq> ls 
-    \<and> currentProc C s \<triangleq> f \<and> f ls = DbOperation operation  ls' \<and> currentTransaction C s \<triangleq> t \<and> querySpec (prog C) operation  (getContext C s) res \<and> visibleCalls C s \<triangleq> vis)"
-  by (auto simp add: precondition_def intro: step.intros elim!: step_elims)
-
-
-
-lemma precondition_return:
-  "precondition (s, AReturn res) C = (\<exists>ls f. localState C s \<triangleq> ls \<and> currentProc C s \<triangleq> f \<and> f ls = Return res \<and> currentTransaction C s = None)"
-  by (auto simp add: precondition_def intro: step.intros elim!: step_elims)
-
-lemma precondition_fail:
-  "precondition (s, AFail) C = (\<exists>ls. localState C s \<triangleq> ls)" \<comment> \<open>failures occur wherever something is running ;)\<close>
-  by (auto simp add: precondition_def intro: step.intros elim!: step_elims)
-
-lemma precondition_invcheck:
-  "precondition (s, AInvcheck res) C \<longleftrightarrow> (res = invariant (prog C) (invContext C))"
-  by (auto simp add: precondition_def step_simps intro: step.intros elim!: step_elims)
-
-
-
-lemma commutativePreservesPrecondition:
-  assumes preconditionHolds: "precondition (sb,b) B"
-    and differentSessions[simp]: "sa \<noteq> sb"
-    and aIsInTransaction: "currentTransaction A sa \<triangleq> tx"
-    and txIsUncommitted: "transactionStatus A tx \<triangleq> Uncommitted"
-    and aIsInLocal: "localState A sa \<triangleq> lsa"
-    and aIsNotCommit: "a \<noteq> AEndAtomic"
-    and exec: "A ~~ (sa, a) \<leadsto> B"
-    and wellFormed: "state_wellFormed A"
-  shows "precondition (sb,b) A"
-proof -
-
-  have origin_inv: "dom (callOrigin A) = dom (calls A)"
-    by (simp add: wellFormed wellFormed_callOrigin_dom)
-
-  have visibleCalls_inv: "\<And>s vis. visibleCalls A s \<triangleq> vis \<Longrightarrow> vis \<subseteq> dom (calls A)"
-    by (simp add: wellFormed wellFormed_visibleCallsSubsetCalls_h(2))
-
-  from exec
-  have committed_same: "transactionStatus A t \<triangleq> Committed \<longleftrightarrow> transactionStatus B t \<triangleq> Committed" for t
-    using aIsNotCommit committed_same by blast
-
-  from exec
-  have callOrigin_same_committed: "callOrigin A c \<triangleq> tx \<longleftrightarrow> callOrigin B c \<triangleq> tx" if "transactionStatus A tx \<triangleq> Committed " for c tx
-    using callOrigin_same_committed that wellFormed by blast    
-
-  from exec
-  have happensBefore_same_committed2: "(x,y) \<in> happensBefore A  \<longleftrightarrow> (x,y) \<in> happensBefore B" 
-    if "transactionStatus A tx \<triangleq> Committed " 
-      and "callOrigin A y \<triangleq> tx"
-    for tx x y
-    using that happensBefore_same_committed2 wellFormed by blast 
-
-  show ?thesis
-  proof (cases b)
-    case ALocal
-    show ?thesis using precondition_alocal unchangedInTransaction
-      by (metis ALocal differentSessions exec preconditionHolds) 
-
-  next
-    case (ANewId x2)
-    with preconditionHolds
-    obtain ls f ls' ls''
-      where 1: "localState B sb \<triangleq> ls" 
-        and 2: "currentProc B sb \<triangleq> f" 
-        and 3: "generatedIds B (to_nat x2) = None" 
-        and 4: "f ls = NewId ls'"
-        and 6: "uniqueIds x2 = {to_nat x2}"
-        and 7: "ls' x2 \<triangleq> ls''"
-      by (auto simp add: precondition_newid)
-    have 5: "generatedIds A (to_nat x2) = None"
-      using generatedIds_mono2_rev[OF 3 exec] by blast
-    then show ?thesis
-      by (metis "1" "2" 4 6 7 ANewId differentSessions exec precondition_newid unchangedInTransaction(1) unchangedInTransaction(2)) 
-  next
-    case (ABeginAtomic tx snapshot)
-    with preconditionHolds obtain ls f ls' vis
-      where 1: "localState B sb \<triangleq> ls"
-        and 2: "currentProc B sb \<triangleq> f"
-        and 3: "f ls = BeginAtomic ls'"
-        and 4: "currentTransaction B sb = None"
-        and 5: "transactionStatus B tx = None"
-        and 6: "chooseSnapshot snapshot vis B"
-        and 7: "visibleCalls B sb \<triangleq> vis"
-      by (auto simp add: precondition_beginAtomic)
-    have tx_none: "transactionStatus A tx = None" using transactionStatus_mono' 5 exec by blast 
-    show ?thesis 
-      using exec differentSessions differentSessions[symmetric] 1 2 3 4 5 6 7 tx_none txIsUncommitted wellFormed 
-      by (auto simp add: wellFormed_callOrigin_dom2 aIsInTransaction aIsNotCommit step.simps \<open>b = ABeginAtomic tx snapshot\<close> precondition_beginAtomic elim!: chooseSnapshot_unchanged_precise split: if_splits)
-
-  next
-    case AEndAtomic
-    then show ?thesis
-      by (metis differentSessions exec preconditionHolds precondition_endAtomic unchangedInTransaction(1) unchangedInTransaction(2) unchangedInTransaction(3))
-  next
-    case (ADbOp callId operation res)
-    with preconditionHolds obtain ls f ls' vis t 
-      where 1: "calls B callId = None"
-        and 2: "localState B sb \<triangleq> ls"
-        and 3: "currentProc B sb \<triangleq> f"
-        and 4: "f ls = DbOperation operation  ls'"
-        and 5: "currentTransaction B sb \<triangleq> t"
-        and 6: "querySpec (prog B) operation  (getContext B sb) res"
-        and 7: "visibleCalls B sb \<triangleq> vis"
-      by (auto simp add: precondition_dbop)
-    moreover have "calls A callId = None"
-      using "1" calls_mono' exec by blast   
-    moreover have "prog B = prog A"
-      using exec prog_inv by auto  
-    moreover have "getContext B sb = getContext A sb"
-      by (metis aIsInTransaction differentSessions exec unchangedInTransaction_getContext visibleCalls_inv) 
-    ultimately show ?thesis  using unchangedInTransaction
-      by (smt ADbOp aIsInTransaction differentSessions exec precondition_dbop)
-
-  next
-    case (AInvoc proc)
-    with preconditionHolds 
-      have "invocationOp B sb = None"
-        and "localState B sb = None"
-        and "uniqueIds proc \<subseteq> knownIds B"
-      by (auto simp add: precondition_invoc)
-    moreover have "invocationOp A sb = None"
-      using aIsInTransaction calculation(1) differentSessions exec unchangedInTransaction(5) by fastforce
-
-    ultimately show ?thesis using unchangedInTransaction
-      by (smt AInvoc aIsInTransaction differentSessions exec precondition_invoc prog_inv)
-  next
-    case (AReturn x8)
-    then show ?thesis
-      by (metis differentSessions exec preconditionHolds precondition_return unchangedInTransaction(1) unchangedInTransaction(2) unchangedInTransaction(3)) 
-  next
-    case AFail
-    then show ?thesis
-      by (metis differentSessions exec preconditionHolds precondition_fail unchangedInTransaction(1))
-  next
-    case (AInvcheck res)
-    with preconditionHolds 
-    have 2: "res = invariant (prog B) (invContext B)"
-      by (auto simp add: precondition_invcheck)
-
-    have invContextSame: "(invContext A) = (invContext B)"
-      using aIsInTransaction aIsNotCommit exec invContextSnapshot_same txIsUncommitted wellFormed by blast
-
-    have "precondition (sb, AInvcheck res) A"  
-      using prog_inv[OF exec] by (auto simp add: precondition_invcheck  committed_same 2 invContextSame)
-
-    then show ?thesis
-      using AInvcheck by blast  
-
-  qed
-qed
-
-
-lemma commutative_ALocal_other:
-  assumes a1: "sa \<noteq> sb"
-  shows "commutativeS S (sa, ALocal) (sb, a)"
-  by (cases a, auto simp add: commutativeS_def steps_simps steps_empty a1 a1[symmetric] fun_upd_twist elim!: chooseSnapshot_unchanged_precise)
-
-
-lemma commutative_other_ALocal:
-  assumes a1: "sa \<noteq> sb"
-  shows "commutativeS S (sa, a) (sb, ALocal)"
-  using assms commutativeS_switchArgs  by (metis commutative_ALocal_other)
-
-
-
-lemma step_existsH:
-  "\<lbrakk>precondition a A; \<And>B. A ~~ a \<leadsto> B \<Longrightarrow> P B \<rbrakk> \<Longrightarrow> \<exists>B. (A ~~ a \<leadsto> B) \<and> P B"
-  using usePrecondition by blast
-
-
-lemma commutative_Dbop_other:
-  assumes a1[simp]: "sa \<noteq> sb"
-    and a2: "state_wellFormed S"
-  shows "commutativeS S (sa, ADbOp c operation res) (sb, a)"
-proof (cases a)
-  case ALocal
-  then show ?thesis  by (simp add: commutative_other_ALocal)
-next
-  case (ANewId x2)
-  then show ?thesis by (auto simp add: steps_empty commutativeS_def steps_appendFront a1[symmetric]  step_simps fun_upd_twist)
-
-
-next
-  case AEndAtomic
-  then show ?thesis by (auto simp add: steps_empty commutativeS_def steps_appendFront a1[symmetric]  step_simps fun_upd_twist)
-next
-  case AFail
-  then show ?thesis by (auto simp add: steps_empty commutativeS_def steps_appendFront  a1[symmetric]  step_simps fun_upd_twist)
-next
-  case (AInvoc p)
-  show ?thesis 
-  proof (induct rule: show_commutativeS_pres)
-    case (preBfront s1)
-    then show ?case 
-      by (auto simp add: AInvoc precondition_invoc step_simps split: if_splits)
-  next
-    case (preAfront s1)
-    then show ?case 
-      by (auto simp add: AInvoc precondition_dbop step_simps)
-  next
-    case (preAback s1)
-    then show ?case 
-      by (auto simp add: AInvoc precondition_dbop step_simps)
-  next
-    case (preBback s1)
-    then show ?case 
-      by (auto simp add: AInvoc precondition_invoc step_simps)
-  next
-    case (commute s1 s2 s1' s2')
-    then show ?case 
-      by (auto simp add: AInvoc commutativeS_def steps_appendFront a1[symmetric]  step_simps fun_upd_twist)
-  qed
-
-next
-  case (AReturn x8)
-  show ?thesis 
-    by (rule show_commutativeS_pres,
-        auto simp add: AReturn precondition_def commutativeS_def steps_appendFront a1[symmetric]  step_simps fun_upd_twist)
-
-next
-  case (AInvcheck res)
-  show ?thesis 
-    by (rule show_commutativeS_pres, auto simp add: a2 AInvcheck precondition_def commutativeS_def steps_appendFront a1[symmetric]  step_simps fun_upd_twist subset_eq invContextH_simps  wellFormed_currentTransactionUncommitted   invContext_unchanged_happensBefore     invContext_unchanged_happensBefore2 
- wellFormed_callOrigin_dom3 wellFormed_currentTransaction_unique_h(2))
-
-
-next
-  case (ADbOp c' operation'  res')
-  show ?thesis 
-    by (rule show_commutativeS_pres2; insert ADbOp a2,
-        auto simp add: precondition_dbop a1[symmetric] step_simps 
-        wellFormed_visibleCallsSubsetCalls2 state_ext differentIds_dbop 
-        getContextH_visUpdate getContextH_callsUpdate
-        split: if_splits)
-next
-next
-  case (ABeginAtomic tx txns)
-  then have a_def[simp]: "a = ABeginAtomic tx txns" .
-      \<comment> \<open>case (APull txns)\<close>
-  show ?thesis
-  proof (induct rule: show_commutativeS_pres2)
-    case (preBfront s1)
-    then show "precondition (sb, a) S" 
-      using a2 by (auto simp add: wellFormed_callOrigin_dom2 wellFormed_currentTransactionUncommitted precondition_dbop precondition_beginAtomic step_simps split: if_splits elim!: chooseSnapshot_unchanged_precise)
-
-  next
-    case (preAfront s1)
-    then show "precondition (sa, ADbOp c operation res) S" 
-      by (auto simp add: precondition_dbop precondition_beginAtomic step_simps)
-  next
-    case (preAback s1)
-    then show "precondition (sa, ADbOp c operation res) s1" 
-      by (auto simp add: precondition_dbop precondition_beginAtomic step_simps)
-  next
-    case (preBback s1)
-    then show "precondition (sb, a) s1" 
-      using a2 by (auto simp add: wellFormed_currentTransaction_unique_h(2) wellFormed_callOrigin_dom2 precondition_dbop precondition_beginAtomic step_simps split: if_splits elim!: chooseSnapshot_unchanged_precise)
-      
-
-  next
-    case (commute s1 s2 s1' s2')
-    then have step1: "S ~~ (sa, ADbOp c operation res) \<leadsto> s1"
-      and step2: "s1 ~~ (sb, ABeginAtomic tx txns) \<leadsto> s2"
-      and step3: "S ~~ (sb, ABeginAtomic tx txns) \<leadsto> s1'"
-      and step4: "s1' ~~ (sa, ADbOp c operation  res) \<leadsto> s2'"
-      by auto
-    show "s2 = s2'" 
-      by (insert step1, auto simp add: step_simps,
-          insert step3, auto simp add: step_simps,
-          insert step2, auto simp add: step_simps,
-          insert step4, auto simp add: step_simps,
-          auto simp add: step_simps a1[symmetric] state_updates_normalize  intro!: show_state_calls_eq)
-  qed
-qed
-
-lemma commutative_newId_other:
-  assumes a1[simp]: "sa \<noteq> sb"
-    and a2: "state_wellFormed S"
-  shows "commutativeS S (sa, ANewId uid) (sb, a)"
-proof (cases a)
-  case ALocal
-  then show ?thesis by (simp add: commutative_other_ALocal)
-next
-  case (ANewId x2)
-  then show ?thesis by (auto simp add: commutativeS_def steps_appendFront a1[symmetric]  step_simps fun_upd_twist insert_commute)
-next
-  case (ABeginAtomic x3)
-  then show ?thesis by (auto simp add: steps_empty commutativeS_def steps_appendFront a1[symmetric]  step_simps fun_upd_twist insert_commute elim!: chooseSnapshot_unchanged_precise)
-
-next
-  case AEndAtomic
-  then show ?thesis by (auto simp add: steps_empty commutativeS_def steps_appendFront a1[symmetric]  step_simps fun_upd_twist insert_commute)
-next
-  case (ADbOp )
-  then show ?thesis
-    using a1 a2 commutativeS_switchArgs commutative_Dbop_other by metis
-next
-  case (AInvoc )
-  then show ?thesis by (auto simp add: steps_empty commutativeS_def steps_appendFront a1[symmetric]  step_simps fun_upd_twist insert_commute)
-next
-  case (AReturn x8)
-  then show ?thesis by (auto simp add: steps_empty commutativeS_def steps_appendFront a1[symmetric]  step_simps fun_upd_twist insert_commute)
-next
-  case AFail
-  then show ?thesis by (auto simp add: steps_empty commutativeS_def steps_appendFront a1[symmetric]  step_simps fun_upd_twist insert_commute)
-next
-  case (AInvcheck x10)
-  then show ?thesis by (auto simp add: steps_empty commutativeS_def steps_appendFront a1[symmetric]  step_simps fun_upd_twist insert_commute)
-qed
-
-lemma commutative_fail_other:
-  assumes a1[simp]: "sa \<noteq> sb"
-    and a2: "state_wellFormed S"
-  shows "commutativeS S (sa, AFail) (sb, a)"
-  by (cases a, auto simp add: steps_empty commutativeS_def steps_appendFront a1[symmetric]  step_simps fun_upd_twist insert_commute elim!: chooseSnapshot_unchanged_precise)
-
-
-
-lemma commutative_beginAtomic_other:
-  assumes a1[simp]: "sa \<noteq> sb"
-    and a2: "state_wellFormed S"
-    and no_end_atomic: "a \<noteq> AEndAtomic" 
-  shows "commutativeS S (sa, ABeginAtomic t newTxns) (sb, a)"
-proof -
-  have a1'[simp]: "sb \<noteq> sa" using a1 ..
-  show "?thesis"
-  proof (cases a)
-    case ALocal
-    then show ?thesis
-      by (simp add: commutative_other_ALocal)
-  next
-    case (ANewId x2)
-    then show ?thesis
-      using a1 a2 commutativeS_switchArgs commutative_newId_other
-      by metis 
-  next
-    case (ABeginAtomic t txns)
-    show ?thesis 
-      by (rule show_commutativeS, 
-        auto simp add: ABeginAtomic step_simps contra_subsetD split: if_splits elim!: chooseSnapshot_unchanged_precise, 
-        subst state_ext;
-        auto simp add: ABeginAtomic step_simps contra_subsetD split: if_splits elim!: chooseSnapshot_unchanged_precise)
-
-
-  next
-    case AEndAtomic \<comment> \<open>this is not commutative, since the transaction committed could be included in ht next snapshot\<close>
-    then show ?thesis
-      using no_end_atomic by auto 
-  next
-    case (ADbOp )
-    then show ?thesis
-      using a1 a2 commutativeS_switchArgs commutative_Dbop_other by metis 
-        (**next
-  case (APull x6)
-  then show ?thesis 
-  by (auto simp add: a2 commutativeS_def steps_appendFront a1[symmetric]  step_simps fun_upd_twist insert_commute,
-    auto, smt mem_Collect_eq option.inject subsetCE transactionStatus.distinct(1))*)
-  next
-    case (AInvoc)
-    then show ?thesis by (auto simp add: steps_empty a2 commutativeS_def steps_appendFront step_simps fun_upd_twist insert_commute split: if_splits elim!: chooseSnapshot_unchanged_precise)
-  next
-    case (AReturn x8)
-    then show ?thesis by (auto simp add: steps_empty a2 commutativeS_def steps_appendFront step_simps fun_upd_twist insert_commute split: if_splits elim!: chooseSnapshot_unchanged_precise)
-  next
-    case AFail
-    then show ?thesis
-      using a1 a2 commutativeS_switchArgs commutative_fail_other by metis 
-  next
-    case (AInvcheck x10)
-    then show ?thesis 
-      by (auto simp add: a2 commutativeS_def steps_appendFront step_simps fun_upd_twist insert_commute invContextH_simps split: if_splits, auto simp add: invContextH_def )
-  qed
-qed
-
-
-lemma commutativeInTransaction:
-  assumes a_is_in_transaction: "currentTransaction S sa \<triangleq> t"
-    and b_is_a_different_session[simp]: "sa \<noteq> sb"
-    and not_endAtomic: "a \<noteq> AEndAtomic"
-    and not_invCheck: "\<not>is_AInvcheck a"
-    and wf[simp]: "state_wellFormed S"
-  shows "commutativeS S (sa, a) (sb, b)"
-proof (cases a)
-  case ALocal
-  then show ?thesis 
-    by (simp add: commutative_ALocal_other)
-next
-  case (ANewId x2)
-  then show ?thesis
-    by (simp add: commutative_newId_other) 
-next
-  case (ABeginAtomic x3)
-  then show ?thesis  
-    by (auto simp add: commutativeS_def steps_appendFront step_simps a_is_in_transaction,
-        metis a_is_in_transaction b_is_a_different_session option.simps(3) unchangedInTransaction(3))
-next
-  case AEndAtomic
-  then show ?thesis using not_endAtomic by simp
-next
-  case (ADbOp)
-  then show ?thesis
-    by (simp add: commutative_Dbop_other)  
-next
-  case (AInvoc)
-  then show ?thesis 
-    by (auto simp add: commutativeS_def steps_appendFront,
-        metis a_is_in_transaction local.wf option.distinct(1) preconditionI precondition_invoc wellFormed_invoc_notStarted(1),
-        metis a_is_in_transaction b_is_a_different_session local.wf option.distinct(1) preconditionI precondition_invoc unchangedInTransaction(5) wellFormed_invoc_notStarted(1))
-next
-  case (AReturn x8)
-  then show ?thesis   
-    by (auto simp add: commutativeS_def steps_appendFront step_simps a_is_in_transaction,
-        metis a_is_in_transaction b_is_a_different_session option.distinct(1) unchangedInTransaction(3))
-
-next
-  case AFail
-  then show ?thesis
-    by (simp add: commutative_fail_other)  
-next
-  case (AInvcheck res)
-  then show ?thesis
-    using is_AInvcheck_def not_invCheck by auto   
-qed
-
-
-
-lemma move_transaction:
-  assumes a_is_in_transaction: "currentTransaction S sa \<triangleq> t"
-    and b_is_a_different_session[simp]: "sa \<noteq> sb"
-    and not_endAtomic: "a \<noteq> AEndAtomic"
-    and not_invCheck: "\<not>is_AInvcheck a"
-    and wf[simp]: "state_wellFormed S"
-  shows "(S ~~ [(sa,a),(sb,b)] \<leadsto>* T) 
-   \<longleftrightarrow> (S ~~ [(sb,b),(sa,a)] \<leadsto>* T)"
-proof (rule useCommutativeS)   
-  show "commutativeS S (sa, a) (sb, b)"
-    by (simp add: a_is_in_transaction commutativeInTransaction not_endAtomic not_invCheck)
-qed
-
-lemma move_transaction2:
-  assumes a_is_in_transaction: "currentTransaction S (get_invoc a) \<triangleq> t"
-    and b_is_a_different_session[simp]: "get_invoc a \<noteq> get_invoc b"
-    and not_endAtomic: "get_action a \<noteq> AEndAtomic"
-    and not_invCheck: "\<not>is_AInvcheck (get_action a)"
-    and wf[simp]: "state_wellFormed S"
-  shows "(S ~~ a#b#xs \<leadsto>* T) 
-   \<longleftrightarrow> (S ~~ b#a#xs \<leadsto>* T)"
-proof -
-  have "(S ~~ a#b#xs \<leadsto>* T) \<longleftrightarrow> (\<exists>S'. (S ~~ [a,b] \<leadsto>* S') \<and> (S' ~~ xs \<leadsto>* T))"
-    by (auto simp add: steps_appendFront steps_empty)
-  moreover have "... \<longleftrightarrow> (\<exists>S'. (S ~~ [b,a] \<leadsto>* S') \<and> (S' ~~ xs \<leadsto>* T))"
-    by (metis a_is_in_transaction b_is_a_different_session local.wf move_transaction not_endAtomic prod.collapse not_invCheck)
-  moreover have "... \<longleftrightarrow> (S ~~ b#a#xs \<leadsto>* T)" 
-    by (auto simp add: steps_appendFront steps_empty)
-  ultimately show ?thesis
-    by blast 
-qed   
-
-
-
-
-
-
-lemma one_compaction_step:
-  assumes splitTrace: "tr = (s, ABeginAtomic tx ntxns) # txa @ x # rest" 
-    and txaInTx: "\<And>st at. (st,at)\<in>set txa \<Longrightarrow> st=s \<and> at \<noteq> AEndAtomic \<and> at \<noteq> AFail \<and> \<not> is_AInvcheck at"
-    and xOutside: "get_invoc x \<noteq> s"
-    and wf: "state_wellFormed s_init"
-    and no_endAtomic: "get_action x \<noteq> AEndAtomic"
-  shows "(s_init ~~ tr \<leadsto>* C)  \<longleftrightarrow> (s_init ~~ x # (s, ABeginAtomic tx ntxns) # txa @ rest \<leadsto>* C)"
-  using splitTrace txaInTx xOutside no_endAtomic  proof (induct txa arbitrary: tr x rest rule: rev_induct)
-  case Nil
-
-  have "(s_init ~~ tr \<leadsto>* C) 
-      = (s_init ~~ (s, ABeginAtomic tx ntxns) # x # rest \<leadsto>* C)" 
-    using Nil by simp
-  moreover have "... = (\<exists>S'. (s_init ~~ [(s, ABeginAtomic tx ntxns), x] \<leadsto>* S') \<and> (S' ~~ rest \<leadsto>* C))"
-    by (auto simp add: steps_appendFront steps_empty)
-  moreover have "... = (\<exists>S'. (s_init ~~ [x, (s, ABeginAtomic tx ntxns)] \<leadsto>* S') \<and> (S' ~~ rest \<leadsto>* C))"
-    using useCommutativeS[OF commutative_beginAtomic_other[OF \<open>get_invoc x \<noteq> s\<close>[symmetric] wf \<open>get_action x \<noteq> AEndAtomic\<close>]]
-    by simp
-  moreover have "... = ( s_init ~~ x # (s, ABeginAtomic tx ntxns) # [] @ rest \<leadsto>* C)"
-    by (auto simp add: steps_appendFront steps_empty)
-
-  ultimately show ?case by auto
-next
-  case (snoc a as)
-
-  have "(s_init ~~ x # (s, ABeginAtomic tx ntxns) # (as @ [a]) @ rest \<leadsto>* C)
-      = (s_init ~~ x # (s, ABeginAtomic tx ntxns) # as @ ([a] @ rest) \<leadsto>* C)"
-    by simp
-  moreover have "... = (s_init ~~ (s, ABeginAtomic tx ntxns) # as @ [x] @ ([a] @ rest) \<leadsto>* C)"
-    using snoc.hyps by (metis append_Cons append_Nil butlast_snoc in_set_butlastD snoc.prems) 
-  moreover have "... = (s_init ~~ (s, ABeginAtomic tx ntxns) # as @ x # a # rest \<leadsto>* C)"
-    by simp
-  moreover have "... = (\<exists>S'. (s_init ~~ (s, ABeginAtomic tx ntxns) # as \<leadsto>* S') \<and> (S' ~~  x # a # rest \<leadsto>* C))"
-    by (auto simp add:  steps_append steps_appendFront)
-  moreover have "... = (\<exists>S'. (s_init ~~ (s, ABeginAtomic tx ntxns) # as \<leadsto>* S') \<and> (S' ~~  a # x # rest \<leadsto>* C))" (is ?eq1)
-  proof -
-    have "(S' ~~ x # a # rest \<leadsto>* C)
-          \<longleftrightarrow> (S' ~~ a # x # rest \<leadsto>* C)" 
-      if "(s_init ~~ (s, ABeginAtomic tx ntxns) # as \<leadsto>* S')"
-      for S'
-    proof (rule move_transaction2[symmetric])
-      have [simp]: "get_invoc a = s" using snoc
-        by (metis list.set_intros(1) prod.collapse rotate1.simps(2) set_rotate1) 
-      show "currentTransaction S' (get_invoc a) \<triangleq> tx" 
-        using currentTransaction_unchangedInternalSteps3
-        by (metis \<open>get_invoc a = s\<close> butlast_snoc in_set_butlastD local.wf snoc.prems(2) that) 
-      show "get_invoc a \<noteq> get_invoc x"
-        using snoc
-        by (metis list.set_intros(1) rotate1.simps(2) set_rotate1 surjective_pairing) 
-      show "get_action a \<noteq> AEndAtomic"
-        using snoc 
-        by (metis list.set_intros(1) rotate1.simps(2) set_rotate1 surjective_pairing)  
-      show "state_wellFormed S'"
-        using wf that by (rule state_wellFormed_combine, 
-            insert snoc.prems(2), fastforce)
-      show " \<not> is_AInvcheck (get_action a)"
-        by (metis list.set_intros(1) prod.collapse rotate1.simps(2) set_rotate1 snoc.prems(2))
-    qed
-    then show ?eq1 by blast
-  qed
-  moreover have "... = (s_init ~~ (s, ABeginAtomic tx ntxns) # as @ a # x # rest \<leadsto>* C)"  
-    by (auto simp add: steps_append steps_appendFront)
-  moreover have "... = (s_init ~~ (s, ABeginAtomic tx ntxns) # (as @ [a]) @ x # rest \<leadsto>* C)"  
-    by auto
-  ultimately show ?case
-    using snoc.prems(1) by blast 
-qed    
-
-
-lemma one_compaction_step2:
-  assumes splitTrace: "tr = trStart @ (s, ABeginAtomic tx ntxns) # txa @ x # rest" 
-    and txaInTx: "\<And>st at. (st,at)\<in>set txa \<Longrightarrow> st=s \<and> at \<noteq> AEndAtomic \<and> at \<noteq> AFail \<and> \<not> is_AInvcheck at"
-    and xOutside: "get_invoc x \<noteq> s"
-    and wf: "state_wellFormed s_init"
-    and no_endatomic: "get_action x \<noteq> AEndAtomic"
-    and noFail: "\<And>i. (i, AFail) \<notin> set tr"
-  shows "(s_init ~~ tr \<leadsto>* C)  \<longleftrightarrow> (s_init ~~ trStart @ x # (s, ABeginAtomic tx ntxns) # txa @ rest \<leadsto>* C)"
-proof 
-  assume "s_init ~~ tr \<leadsto>* C"
-  with steps_append 
-  obtain S_mid where "s_init ~~ trStart \<leadsto>* S_mid" and "S_mid ~~ (s, ABeginAtomic tx ntxns) # txa @ x # rest \<leadsto>* C"
-    using splitTrace by blast
-
-  have "state_wellFormed S_mid"
-    using \<open>s_init ~~ trStart \<leadsto>* S_mid\<close> local.wf noFail splitTrace state_wellFormed_combine by fastforce
-
-
-  from \<open>S_mid ~~ (s, ABeginAtomic tx ntxns) # txa @ x # rest \<leadsto>* C\<close>
-  have "S_mid ~~ x # (s, ABeginAtomic tx ntxns) # txa @ rest \<leadsto>* C"
-    using \<open>state_wellFormed S_mid\<close> no_endatomic one_compaction_step txaInTx xOutside by blast
-
-  then show "s_init ~~ trStart @ x # (s, ABeginAtomic tx ntxns) # txa @ rest \<leadsto>* C"
-    using \<open>s_init ~~ trStart \<leadsto>* S_mid\<close> steps_append2 by blast
-next \<comment> \<open>Other direction is very similar:\<close>
-  assume "s_init ~~ trStart @ x # (s, ABeginAtomic tx ntxns) # txa @ rest \<leadsto>* C"
-  with steps_append 
-  obtain S_mid where "s_init ~~ trStart \<leadsto>* S_mid" and "S_mid ~~ x # (s, ABeginAtomic tx ntxns) # txa @ rest \<leadsto>* C"
-    by blast
-
-  have "state_wellFormed S_mid"
-    using \<open>s_init ~~ trStart \<leadsto>* S_mid\<close> local.wf noFail splitTrace state_wellFormed_combine by fastforce
-
-  from \<open>S_mid ~~ x # (s, ABeginAtomic tx ntxns) # txa @ rest \<leadsto>* C\<close>
-  have "S_mid ~~ (s, ABeginAtomic tx ntxns) # txa @ x # rest \<leadsto>* C"
-    using \<open>state_wellFormed S_mid\<close> no_endatomic one_compaction_step txaInTx xOutside by blast
-
-  then show "s_init ~~ tr \<leadsto>* C"
-    using \<open>s_init ~~ trStart \<leadsto>* S_mid\<close> splitTrace steps_append2 by blast
-qed
-
-
-lemma one_compaction_step3:
-  assumes splitTrace: "tr = trStart @ (s, ABeginAtomic tx ntxns) # txa @ x # rest" 
-    and splitTrace': "tr' = trStart @ x # (s, ABeginAtomic tx ntxns) # txa @ rest"
-    and txaInTx: "\<And>st at. (st,at)\<in>set txa \<Longrightarrow> st=s \<and> at \<noteq> AEndAtomic \<and> at \<noteq> AFail \<and> \<not> is_AInvcheck at"
-    and xOutside: "get_invoc x \<noteq> s"
-    and wf: "state_wellFormed s_init"
-    and no_endatomic: "get_action x \<noteq> AEndAtomic"
-    and noFail: "\<And>i. (i, AFail) \<notin> set tr"
-  shows "(s_init ~~ tr \<leadsto>* C)  \<longleftrightarrow> (s_init ~~ tr' \<leadsto>* C)"
-  using local.wf one_compaction_step2 splitTrace splitTrace' txaInTx xOutside no_endatomic noFail by blast 
-
-
-
-
 definition canSwap :: "'ls itself \<Rightarrow> ('proc::valueType, 'operation, 'any::valueType)  action \<Rightarrow> ('proc, 'operation, 'any) action \<Rightarrow> bool" where
-  "canSwap t a b \<equiv> (\<forall>(C1::('proc, 'ls, 'operation, 'any) state) C2 s1 s2. 
-      s1\<noteq>s2 \<and> (C1 ~~ [(s1,a),(s2,b)] \<leadsto>* C2) \<and> state_wellFormed C1 \<longrightarrow> (C1 ~~ [(s2,b),(s1,a)] \<leadsto>* C2))"
-
-lemma show_canSwap:
-  assumes "\<And>(C1::('proc::valueType, 'ls, 'operation, 'any::valueType) state) C2 C3 s1 s2. \<lbrakk>s1 \<noteq> s2; C1 ~~ (s1,a) \<leadsto> C2; C2 ~~ (s2,b) \<leadsto> C3; state_wellFormed C1\<rbrakk> \<Longrightarrow> \<exists>C. (C1 ~~ (s2,b) \<leadsto> C) \<and> (C ~~ (s1,a) \<leadsto> C3)"
-  shows "canSwap (t::'ls itself) a b"
-proof (auto simp add: canSwap_def)
-  fix C1 C3 :: "('proc, 'ls, 'operation, 'any) state"
-  fix s1 s2
-  assume a0: "s1 \<noteq> s2"
-    and a1: "C1 ~~ [(s1, a), (s2, b)] \<leadsto>* C3"
-    and a2: "state_wellFormed C1"
-
-  from a1 obtain C2
-    where a1': "C1 ~~ (s1,a) \<leadsto> C2" and a1'': "C2 ~~ (s2,b) \<leadsto> C3"
-    using steps_appendFront steps_single by blast
-
-
-  show "C1 ~~ [(s2, b), (s1, a)] \<leadsto>* C3"
-  proof (subst steps.simps, clarsimp simp add: steps_empty steps_single, rule assms)
-    show "s1 \<noteq> s2" using a0.
-    show "C1 ~~ (s1, a) \<leadsto> C2" using a1'.
-    show "C2 ~~ (s2,b) \<leadsto> C3" using a1''.
-    show "state_wellFormed C1" using a2.
-  qed
-qed
-       
-lemma show_canSwap':
-  assumes "x = a" 
-    and"\<And>(C1::('proc::valueType, 'ls, 'operation, 'any::valueType) state) C2 C3 s1 s2. \<lbrakk>s1 \<noteq> s2; C1 ~~ (s1,a) \<leadsto> C2; C2 ~~ (s2,b) \<leadsto> C3; state_wellFormed C1\<rbrakk> \<Longrightarrow> \<exists>C. (C1 ~~ (s2,b) \<leadsto> C) \<and> (C ~~ (s1,a) \<leadsto> C3)"
-  shows "canSwap (t::'ls itself) x b"
-  by (simp add: assms show_canSwap)
-
-method prove_canSwap = (
-    rule show_canSwap, 
-    auto simp add: step_simps state_updates_normalize fun_upd_twist intro!: show_state_calls_eq elim!: chooseSnapshot_unchanged_precise)
-
-method prove_canSwap' = (
-    rule show_canSwap', 
-    auto simp add: step_simps state_updates_normalize fun_upd_twist intro!: show_state_calls_eq elim!: chooseSnapshot_unchanged_precise)
-method prove_canSwap'' = (
-    rule show_canSwap', 
-    auto del: ext  simp add: wellFormed_callOrigin_dom2 step_simps wellFormed_currentTransactionUncommitted state_updates_normalize fun_upd_twist intro!: show_state_calls_eq ext split: if_splits elim!: chooseSnapshot_unchanged_precise)
-
-lemma commutativeS_canSwap:
-  assumes comm: "\<And>(C::('proc::valueType, 'ls, 'operation, 'any::valueType) state) s1 s2. \<lbrakk>s1\<noteq>s2;  state_wellFormed C\<rbrakk> \<Longrightarrow> commutativeS C (s1,a) (s2,b)"
-  shows "canSwap (t::'ls itself) a b"
-proof (auto simp add: canSwap_def)
-  fix C1 C2 :: "('proc, 'ls, 'operation, 'any) state"
-  fix s1 s2
-  assume a0: "s1 \<noteq> s2"
-    and a1: "C1 ~~ [(s1, a), (s2, b)] \<leadsto>* C2"
-and a2: "state_wellFormed C1"
-
-  show "C1 ~~ [(s2, b), (s1, a)] \<leadsto>* C2"
-  proof (subst useCommutativeS)
-    show "commutativeS C1 (s2, b) (s1, a)" 
-      using comm a0  a2 by (simp add: commutativeS_switchArgs)
-    show "C1 ~~ [(s1, a), (s2, b)] \<leadsto>* C2" using a1.
-  qed
-qed
-
-lemma commutativeS_canSwap_sym:
-  assumes comm: "\<And>(C::('proc::valueType, 'ls, 'operation, 'any::valueType) state) s1 s2. \<lbrakk>s1\<noteq>s2;  state_wellFormed C\<rbrakk> \<Longrightarrow> commutativeS C (s1,b) (s2,a)"
-  shows "canSwap (t::'ls itself) a b"
-  by (metis comm commutativeS_canSwap commutativeS_switchArgs)
-
-
-
+  "canSwap t a b \<equiv> (\<forall>(C1::('proc, 'ls, 'operation, 'any) state) C2 i1 i2. 
+      i1\<noteq>i2 \<and> (C1 ~~ [(i1,a),(i2,b)] \<leadsto>* C2) \<and> state_wellFormed C1 \<longrightarrow> (C1 ~~ [(i2,b),(i1,a)] \<leadsto>* C2))"
 
 
 text \<open>We can swap one action over a list of actions with canSwap\<close>
@@ -933,6 +105,44 @@ lemma swapMany_middle':
   by (insert assms, cases a, rule ssubst, assumption, rule swapMany_middle, auto)
 
 
+lemma show_canSwap:
+  assumes "\<And>(C1::('proc::valueType, 'ls, 'operation, 'any::valueType) state) C2 C3 s1 s2. \<lbrakk>s1 \<noteq> s2; C1 ~~ (s1,a) \<leadsto> C2; C2 ~~ (s2,b) \<leadsto> C3; state_wellFormed C1\<rbrakk> \<Longrightarrow> \<exists>C. (C1 ~~ (s2,b) \<leadsto> C) \<and> (C ~~ (s1,a) \<leadsto> C3)"
+  shows "canSwap (t::'ls itself) a b"
+proof (auto simp add: canSwap_def)
+  fix C1 C3 :: "('proc, 'ls, 'operation, 'any) state"
+  fix s1 s2
+  assume a0: "s1 \<noteq> s2"
+    and a1: "C1 ~~ [(s1, a), (s2, b)] \<leadsto>* C3"
+    and a2: "state_wellFormed C1"
+
+  from a1 obtain C2
+    where a1': "C1 ~~ (s1,a) \<leadsto> C2" and a1'': "C2 ~~ (s2,b) \<leadsto> C3"
+    using steps_appendFront steps_single by blast
+
+
+  show "C1 ~~ [(s2, b), (s1, a)] \<leadsto>* C3"
+  proof (subst steps.simps, clarsimp simp add: steps_empty steps_single, rule assms)
+    show "s1 \<noteq> s2" using a0.
+    show "C1 ~~ (s1, a) \<leadsto> C2" using a1'.
+    show "C2 ~~ (s2,b) \<leadsto> C3" using a1''.
+    show "state_wellFormed C1" using a2.
+  qed
+qed
+
+lemma show_canSwap':
+  assumes "x = a" 
+    and"\<And>(C1::('proc::valueType, 'ls, 'operation, 'any::valueType) state) C2 C3 s1 s2. \<lbrakk>s1 \<noteq> s2; C1 ~~ (s1,a) \<leadsto> C2; C2 ~~ (s2,b) \<leadsto> C3; state_wellFormed C1\<rbrakk> \<Longrightarrow> \<exists>C. (C1 ~~ (s2,b) \<leadsto> C) \<and> (C ~~ (s1,a) \<leadsto> C3)"
+  shows "canSwap (t::'ls itself) x b"
+  by (simp add: assms show_canSwap)
+
+method prove_canSwap'' uses simp  = (
+    rule show_canSwap', 
+    auto del: ext  simp add: simp step_simps fun_upd_twist intro!: show_state_calls_eq ext split: if_splits elim!: chooseSnapshot_unchanged_precise)
+
+
+thm wellFormed_callOrigin_dom2  wellFormed_currentTransactionUncommitted state_updates_normalize 
+
+
 
 text "The following are all the relevant cases where canSwap is true:"
 lemma canSwap_cases:
@@ -945,14 +155,71 @@ lemma canSwap_cases:
   shows "canSwap t a b"
 proof (cases b)
   case ALocal
-  then show ?thesis
-    by (simp add: commutativeS_canSwap commutative_other_ALocal)
+  hence [simp]: " b = ALocal" .
+
+  show ?thesis
+  proof (cases a)
+    case ALocal
+    then show ?thesis by prove_canSwap''
+  next
+    case (ANewId x2)
+    then show ?thesis by prove_canSwap''
+  next
+    case (ABeginAtomic x31 x32)
+    then show ?thesis  by prove_canSwap''
+  next
+    case AEndAtomic
+    then show ?thesis  by prove_canSwap''
+  next
+    case (ADbOp x51 x52 x53)
+    then show ?thesis  by prove_canSwap''
+  next
+    case (AInvoc x6)
+    then show ?thesis  by prove_canSwap''
+  next
+    case (AReturn x7)
+    then show ?thesis  by prove_canSwap''
+  next
+    case AFail
+    then show ?thesis  by prove_canSwap''
+  next
+    case (AInvcheck x9)
+    then show ?thesis  by prove_canSwap''
+  qed
 next
   case (ANewId bid)
   then have [simp]: "b = ANewId bid" .
 
   show ?thesis
-    by (simp add: commutativeS_canSwap_sym commutative_newId_other)
+  proof (cases a)
+    case ALocal
+    then show ?thesis  by prove_canSwap''
+  next
+    case (ANewId x2)
+    then show ?thesis  by prove_canSwap''
+  next
+    case (ABeginAtomic x31 x32)
+    then show ?thesis  by prove_canSwap''
+  next
+    case AEndAtomic
+    then show ?thesis  by prove_canSwap''
+  next
+    case (ADbOp x51 x52 x53)
+    then show ?thesis  by prove_canSwap''
+  next
+    case (AInvoc x6)
+    then show ?thesis  by prove_canSwap''
+  next
+    case (AReturn x7)
+    then show ?thesis  by prove_canSwap''
+  next
+    case AFail
+    then show ?thesis  by prove_canSwap''
+  next
+    case (AInvcheck x9)
+    then show ?thesis  by prove_canSwap''
+  qed
+
 next
   case (ABeginAtomic x31 x32)
   then show ?thesis
@@ -961,26 +228,24 @@ next
   case AEndAtomic
   then have [simp]: "b = AEndAtomic" .
   then show ?thesis 
-  proof (cases a; prove_canSwap?)
+  proof (cases a)
     case ALocal
-    then show ?thesis
-      by (simp add: commutativeS_canSwap commutative_ALocal_other)
+    then show ?thesis  by prove_canSwap''
   next
     case (ANewId x2)
-    then show ?thesis
-      by (simp add: commutativeS_canSwap commutative_newId_other) 
+    then show ?thesis  by prove_canSwap''
   next
     case (ABeginAtomic x31 x32)
     then show ?thesis 
-      by prove_canSwap''
+      by (prove_canSwap'' simp:   wellFormed_currentTransactionUncommitted  )
   next
     case AEndAtomic
     then show ?thesis 
       by prove_canSwap''
   next
     case (ADbOp )
-    then show ?thesis
-      by (simp add: commutativeS_canSwap commutative_Dbop_other)
+    then show ?thesis 
+      by prove_canSwap''
   next
     case (AInvoc )
     then show ?thesis
@@ -1008,14 +273,14 @@ next
     then show ?thesis by prove_canSwap''
   next
     case (ABeginAtomic x31 x32)
-    then show ?thesis by prove_canSwap''
+    then show ?thesis by (prove_canSwap'' simp: wellFormed_callOrigin_dom2  wellFormed_currentTransactionUncommitted  )
   next
     case AEndAtomic
     then show ?thesis by prove_canSwap''
   next
     case (ADbOp )
     then show ?thesis
-      by (meson canSwap_def commutative_Dbop_other useCommutativeS)  
+      by (prove_canSwap'' simp:  getContextH_callsUpdate getContextH_visUpdate wellFormed_visibleCallsSubsetCalls2)  
   next
     case (AInvoc )
     then show ?thesis by prove_canSwap''
@@ -1077,8 +342,6 @@ next
   then show ?thesis
     using is_AInvcheck_def no_invcheck_b by auto 
 qed
-
-
 
 
 end
